proofs/x86-64/avx2/ml_dsa_65/common/encoding/signature.ec
@@ -3,7 +3,7 @@ require import AllCore List IntDiv RealExp StdBigop.
 from Jasmin require import JModel_x86.
 
 from JazzEC require import Ml_dsa_65_avx2.
-from JazzEC require import Array256 Array128.
+from JazzEC require import Array256 Array61 Array1536 Array3309.
 from Spec require import GFq Rq Serialization Conversion Parameters VecMat MLDSA_W32_Rep.
 import BitEncoding BitChunking.
 
@@ -11,11 +11,7 @@ import CDR Round Zq.
 
 require import ArrayExtra JWord_extra EclibExtra JWordList.
 
-require import Array640 Array1280.
-
 import VecMat PolyKVec.
-
-require import Array1536 Array3309.
 
 op  decoded_unflatten(a : 'a Array1536.t) =
      KArray.init (fun i => Array256.of_list witness (sub a (256*i) 256)).
@@ -47,13 +43,156 @@ rewrite mapiE 1:/# /= mapiE 1:/# /= initiE 1:/# initiE 1:/# /=.
 by rewrite !get_of_list 1,2:/# /= !nth_sub /#. 
 qed.
 
+lemma decode_hint :
+    w_hint = 55 =>
+    kvec = 6 =>
+    equiv [ HintPackUnpack.hintBitUnpack ~ M.signature____decode_hint :
+       arg{1} = to_list arg{2}.`2 
+     ==>
+      (res{1} = None  => res{2}.`2 = -W64.one) /\
+      (res{1} <> None =>
+         res{2}.`2 = W64.zero /\
+         liftu_wpolykvec (decoded_unflatten res{2}.`1) = oget res{1} /\
+         wpolykvec_urng (decoded_unflatten res{2}.`1) 2)
+   ].
+proof.
+move => whint kvec.
+proc => /=.
+wp; conseq (_: _ ==>
+      (error{1} => ill_formed_hint{2} = W64.one) /\
+      (!error{1} =>
+         ill_formed_hint{2} = W64.zero /\
+   liftu_wpolykvec (decoded_unflatten hints{2}) = h{1} /\
+   wpolykvec_urng (decoded_unflatten hints{2}) 2)).
++ auto => /> error1 h1 h2 error2 He Hne;split;1:smt().
+  move => ?; move : Hne; have ->/= : error1 = false; 1:smt().
+  move => [#] ->?? /=;split;1:by ring.
+  by smt().
+
+(* Initialization *)
+seq 3 2  :
+  (#pre /\
+   !error{1} /\
+   index{1} = previous_true_hints_seen{2} /\
+   (error{1} => ill_formed_hint{2} = W64.one) /\
+   (!error{1} => ill_formed_hint{2} = W64.zero));
+   1: by auto => />.
+
+(* Check for zero *)
+seq 2 5 :
+  (#{/~!error{1}}pre /\
+   index{1} = previous_true_hints_seen{2} /\
+   (error{1} => ill_formed_hint{2} = W64.one) /\
+   (!error{1} => ill_formed_hint{2} = W64.zero) /\
+   (!error{1} =>
+      liftu_wpolykvec (decoded_unflatten hints{2}) = h{1} /\
+      wpolykvec_urng (decoded_unflatten hints{2}) 2)
+  ); last first.
++ while (#post /\
+     y{1} = to_list hint_encoded{2} /\
+     index{1} = encoded_offset {2}); last first.
+   + auto => /> &1 &2 ?Hne?;split; 1: smt().
+     do split;rewrite /SETcc.
+     + move => ??;case (55 <= previous_true_hints_seen{2}) => ?.
+       + rewrite wordP => i ib; rewrite orwE /=;smt(W8.nth_one). 
+       by rewrite Hne 1:/# or0w /truncateu8 /= /#.
+     + case (55 <= previous_true_hints_seen{2}) => ?.
+       + rewrite wordP => Hw; have /= := Hw 0 _;1:smt().
+       by rewrite W8.nth_one /=.
+    by rewrite or0w /truncateu8 /= to_uint_eq /= => ?;smt(W64.to_uint1 W64.to_uint0).
+   case (to_uint (nth witness y{1} index{1}) <> 0).
+   + rcondt {1} ^if;1: by auto.
+     rcondt {2} ^if; 1: by  auto => /> *; rewrite to_uint_eq to_uint_zeroextu64.
+     rcondf {2} ^if; 1: by auto => />;by smt(W64.to_uint1 W64.to_uint0).
+     auto => /> &1 &2 ?????;rewrite /SETcc.
+     case (55 <= encoded_offset{2}) => ?;1: smt(W8.wordP orwE W8.nth_one).
+     by rewrite or0w /truncateu8 /= to_uint_eq /=.
+   + rcondf {1} ^if;1: by auto.
+     rcondf {2} ^if; 1: by auto => /> *;rewrite to_uint_eq  to_uint_zeroextu64 /#.
+     rcondt {2} ^if; 1: by auto => />;by smt(W64.to_uint1 W64.to_uint0).
+     auto => /> &1 &2 ?????;split;rewrite /SETcc.
+     +  case (55 <= encoded_offset{2} + 1) => ?;1: smt(W8.wordP orwE W8.nth_one).
+        by rewrite or0w /truncateu8 /= to_uint_eq /=;by smt(W64.to_uint1 W64.to_uint0).
+     case (55 <= encoded_offset{2} + 1) => ?;2: smt(W64.to_uint1 W64.to_uint0).
+     rewrite wordP => Hw; have /= := Hw 0 _;1:smt().
+     by rewrite W8.nth_one /=.
+
+(* Main loop *)
+while (0 <= i{1} <= kvec /\
+    i{1} = encoded_offset{2} /\
+    y{1} = to_list hint_encoded{2} /\
+   index{1} = previous_true_hints_seen{2} /\
+   (error{1} => ill_formed_hint{2} = W64.one) /\
+  index{1} = previous_true_hints_seen{2} /\
+  (error{1} => ill_formed_hint{2} = W64.one) /\
+  (!error{1} => ill_formed_hint{2} = W64.zero) /\
+  (!error{1} =>
+     forall k, 0 <= k < i{1} =>
+       (liftu_wpolykvec (decoded_unflatten hints{2})).[k] = h{1}.[k] /\
+       wpoly_urng 2 (decoded_unflatten hints{2}).[k])); last first.
++ auto => /> &1 &2 *;do split;1..3:smt().
+  move => e1 h1 d12 eo2 h2 if2 ??????H H0;split.
+  + rewrite tP => k kb.
+    have := H H0 k _;smt().
+  rewrite /wpolykvec_urng allP => k kb.
+  by have := H H0 k _;smt().
+
+seq 0 2 : (#pre /\ decoded_offset{2} = 256*encoded_offset{2});
+  1: by auto => /> &1 &2 ???????;rewrite /(`<<`) /= /#.
+
+(* Set Zero *)
+seq 1 2 : (#pre /\ 
+      (liftu_wpolykvec (decoded_unflatten hints{2})).[i{1}] = h{1}.[i{1}] /\
+      wpoly_urng 2 (decoded_unflatten hints{2}).[i{1}]).
+ + wp; conseq />;1:smt().
+   while {2} (0 <= j{2} <= n /\ 0 <= encoded_offset{2} < kvec /\
+      decoded_offset{2} = encoded_offset{2} * n /\
+     (forall (k : int),
+        0 <= k < encoded_offset{2} =>
+          (liftu_wpolykvec (decoded_unflatten hints{2})).[k] =
+            h{1}.[k] /\
+     wpoly_urng 2 (decoded_unflatten hints{2}).[k]) /\
+     (forall jj, 0 <= jj < j{2} =>
+  (decoded_unflatten hints{2}).[encoded_offset{2}].[jj] = W32.zero)) (n - j{2}); last first.
+   + auto => /> &1 &2 ???????;split;1:smt().
+   move  => h2 j2;split;1:smt().
+   move => ??????H; do split.
+   + move => k kbl kbh.
+     split.
+     + by rewrite mapiE 1:/# get_setE 1:/# ifF 1:/#; smt(KArray.mapiE).
+     by smt(KArray.allP).
+   + rewrite get_setE 1:/# ifT 1:/# tP => k kb.
+    by  rewrite mapiE 1:/# /= Array256.initiE 1:/# /=  mapiE 1:/# /= H 1:/# /=.
+   + rewrite /wpoly_urng allP => k kb /=.
+     by rewrite H /#.
+ + move => &1 _z;auto => /> &2 ???? H H0 ?; do split; 1,2,5:smt().
+   + move => k kbl kbh.
+     have  := H k _;1:smt().
+     rewrite mapiE 1:/# /= tP /wpoly_urng allP => [# HH HH0].
+     split.
+     + rewrite mapiE 1:/# /= tP => kk kkb.
+       rewrite mapiE 1:/# /= initiE 1:/# /= get_of_list 1:/# nth_sub 1:/# /=.
+       by have := HH kk kkb; rewrite  initiE 1:/# /= mapiE 1:/# /= get_of_list 1:/# nth_sub 1:/# /= get_setE /#.
+   +  rewrite allP => kk kkb /=;rewrite initiE 1:/# /= get_of_list 1:/# nth_sub 1:/# /= get_setE 1:/#.
+     have /= := HH0 kk kkb.
+     rewrite initiE 1:/# /= get_of_list 1:/# nth_sub 1:/# /= => HH1.
+     by smt().
+   + move => jj jjbl jjbh.
+     rewrite initiE 1:/# /= get_of_list 1:/# nth_sub 1:/# /=.
+     case (jj = j{2}) => ?.
+     + by rewrite get_setE 1:/# ifT 1:/#.
+     rewrite get_setE 1:/# ifF 1:/#.
+     have /= := H0 jj _;1:smt().
+     by rewrite initiE 1:/# /= get_of_list 1:/# nth_sub /#.
+
+admitted.
+     
 op count_nonzero_coeffs(p : poly) = count (fun c => c = Zq.one) (to_list p).
 
 import Bigint BIA. 
 op count_nonzero_coeffs_kvec(v : polykvec) =
      big predT count_nonzero_coeffs (to_list v).
 
-(* Helper: count ones in first i complete polynomials plus first j coeffs of poly i *)
 op count_nonzero_prefix(v : polykvec) (i j : int) : int =
   big predT count_nonzero_coeffs (take i (to_list v)) +
   (if 0 <= i < kvec then
@@ -64,7 +203,7 @@ lemma count_nonzero_prefix_one(v : coeff Array1536.t) (i j : int)  :
    0 <= i < kvec =>
    0 <= j < n =>
    (decoded_unflatten v).[i].[j] = Zq.one =>
-   count_nonzero_coeffs_kvec (decoded_unflatten v) = w_hint =>
+   count_nonzero_coeffs_kvec (decoded_unflatten v) <= w_hint =>
       count_nonzero_prefix (decoded_unflatten v) i j < w_hint.
 move => ???.
 rewrite /count_nonzero_coeffs_kvec /count_nonzero_prefix ifT 1:/#.
@@ -92,7 +231,7 @@ lemma encode_hint _signature _hint :
     kvec = 6 =>
     equiv [ HintPackUnpack.hintBitPack ~ M.signature____encode_hint :
        wpolykvec_urng (decoded_unflatten hint_0{2}) 2
-    /\ count_nonzero_coeffs_kvec (decoded_unflatten _hint) = w_hint
+    /\ count_nonzero_coeffs_kvec (decoded_unflatten _hint) <= w_hint
     /\ arg{1} = decoded_unflatten _hint
     /\ arg{2}.`1 = _signature
     /\ liftu_wpolykvec (decoded_unflatten arg{2}.`2) =  decoded_unflatten _hint
@@ -124,30 +263,22 @@ seq 3 4 : (#{/~signature{2} = _signature}pre
                signature{2}.[3248 + k] = W8.zero)
    /\ touch_hint _signature signature{2});
    last by auto => />; smt(eq_in_mkseq).
-  by auto => /> &hr; smt(get_setE).
+  by auto => /> &hr; smt(Array3309.get_setE).
   by move => ?;while(true) (61-i); auto => /> /#.
 (* Main nested loops *)
 seq 1 2 : (#{/~i{1}}{i{2}}{index{1}}{hints_written{2}}pre
-    /\ count_nonzero_coeffs_kvec (decoded_unflatten _hint) = w_hint
+    /\ count_nonzero_coeffs_kvec (decoded_unflatten _hint) <= w_hint
    /\ touch_hint _signature signature{2}
    /\ size y{1} = w_hint + kvec
    /\ i{1} = kvec
-   /\ i{2} = kvec
+   /\ i{2} = i{1}
    /\ index{1} = hints_written{2}
-   /\ index{1} = w_hint
-   /\ (forall k, 0 <= k < index{1} =>
-        y{1}.[k] = signature{2}.[3248 + k])
-   /\ (forall k, 0 <= k < kvec =>
-        y{1}.[w_hint + k] = signature{2}.[3248 + w_hint + k])); last first.
-+ auto => /> &1 &2 ????H2.
-  + apply (eq_from_nth W8.zero); 1: by rewrite size_mkseq;smt().
-    move => i ib; rewrite nth_mkseq 1:/# /=. 
-    case (i < w_hint) => ?;1:smt().
-    by have  := H2 (i - w_hint) _; smt().
+   /\ index{1} <= w_hint
+   /\  y{1} = mkseq (fun (i0 : int) => signature{2}.[3248 + i0]) hint_bytes); last by auto.
 + (* Outer loop over polynomials *)
   while (
     wpolykvec_urng (decoded_unflatten hint_0{2}) 2 /\
-    count_nonzero_coeffs_kvec (decoded_unflatten _hint) = w_hint /\
+    count_nonzero_coeffs_kvec (decoded_unflatten _hint) <= w_hint /\
     h{1} = decoded_unflatten _hint /\
     liftu_wpolykvec (decoded_unflatten hint_0{2}) = decoded_unflatten _hint /\           
     size y{1} = hint_bytes /\
@@ -156,23 +287,16 @@ seq 1 2 : (#{/~i{1}}{i{2}}{index{1}}{hints_written{2}}pre
     0 <= index{1} <= w_hint /\
     index{1} = hints_written{2} /\
     index{1} = count_nonzero_prefix (decoded_unflatten _hint) i{1} 0 /\
-    (* Encoding matches for positions written so far *)
-    (forall k, 0 <= k < index{1} =>
-      y{1}.[k] = signature{2}.[3248 + k]) /\
-    (* Cumulative counts match for completed polynomials *)
-    (forall k, 0 <= k < i{1} =>
-       y{1}.[w_hint + k] = signature{2}.[3248 + w_hint + k]) /\
+   y{1} = mkseq (fun (i0 : int) => signature{2}.[3248 + i0]) hint_bytes /\
     touch_hint _signature signature{2} /\
     condition1{2} = (i{2} < 6)
   ); last first.
- + auto => /> &1 &2 ???;do split;1..3,5..7:smt(size_mkseq).
+ + auto => /> &1 &2 ???;do split;1..3,5..6:smt(size_mkseq).
     + by rewrite /count_nonzero_prefix /= !take0 big_nil /#. 
-    + move => y1 c1 i2 s2 ????????H2??;do split;1..2,4..: smt().
-      + by rewrite /count_nonzero_prefix ifF 1:/# /= take_oversize /=;smt(KArray.size_to_list).
   wp. (* Inner while loop *)
   while (
        wpolykvec_urng (decoded_unflatten hint_0{2}) 2 /\
-       count_nonzero_coeffs_kvec (decoded_unflatten _hint) = w_hint /\
+       count_nonzero_coeffs_kvec (decoded_unflatten _hint) <= w_hint /\
         h{1} = decoded_unflatten _hint /\
         liftu_wpolykvec (decoded_unflatten hint_0{2}) = decoded_unflatten _hint /\           
         size y{1} = hint_bytes /\
@@ -183,35 +307,32 @@ seq 1 2 : (#{/~i{1}}{i{2}}{index{1}}{hints_written{2}}pre
         index{1} = count_nonzero_prefix (decoded_unflatten _hint) i{1} j{1} /\
         0 <= j{1} <= 256 /\
         j{1} = j{2} /\
-        (forall k, 0 <= k < index{1} =>
-          y{1}.[k] = signature{2}.[3248 + k]) /\
-        (forall k, 0 <= k < i{1} =>
-          y{1}.[w_hint + k] = signature{2}.[3248 + w_hint + k]) /\
+        y{1} = mkseq (fun (i0 : int) => signature{2}.[3248 + i0]) hint_bytes /\
         touch_hint _signature signature{2} /\
         condition2{2} = (j{2} < 256)
   ); last first.
-  + auto => /> &1 &2 Hrng ????????????  y1 c1 j2 s2 ????????H2??; do split;1..3,8..:smt(size_put).
+  + auto => /> &1 &2 Hrng ?????????  c1 j2 s2 *; do split;1..3,7..:smt(size_put).
     + rewrite /count_nonzero_prefix ifT 1:/#.
-      case (i{2} + 1 = kvec) => ?. 
+      case (i{1} + 1 = kvec) => ?. 
       + rewrite ifF 1:/# /= (take_nth witness) /=;1:smt(KArray.size_to_list).
         by rewrite big_rcons ifT 1:/# (take_oversize j2) ?size_to_list /#.
       rewrite ifT 1:/# (take_nth witness);1:smt(KArray.size_to_list).
       by rewrite big_rcons ifT 1:/# /= take0 /= (take_oversize j2) ?size_to_list /#.
-   + move => k??; rewrite nth_put;smt(get_setE).
-   + move => k??;rewrite nth_put 1:/# /=.
-     case (i{2} = k) => * ;smt(get_setE).
-   + by smt(get_setE).
+   + apply (eq_from_nth witness);1:smt(size_put size_mkseq).
+     move => k; rewrite size_put size_mkseq /max ifT 1:/# /= => kb.
+     by rewrite nth_put 1:/# /=; smt(nth_mkseq Array3309.get_setE).
+   + by smt(Array3309.get_setE).
 
  seq 0 4 : (#pre /\
      to_uint hint_coefficient{2} = asint h{1}.[i{1}].[j{1}]).
- + auto => /> &1 &2 Hrng ? Hh2 ???????????. 
+ + auto => /> &2 Hrng ? Hh2 ?????????. 
    have  /= Hrngp := decoded_unflattenE i{2} j{2} hint_0{2} (fun (ii : W32.t) => 0 <= to_uint ii < 2) _ _ _ _;1..4:smt().
    have  /= Hh2p := decoded_unflattenP i{2} j{2} hint_0{2} _hint (fun (ii : W32.t) => incoeff (to_uint ii)) _ _ _ _;1..4: smt(). 
    rewrite /(`<<`) /= /decoded_unflatten initiE 1:/# /=.
    by rewrite get_of_list 1:/# /= nth_sub 1:/# /=; smt(incoeffK).
 
 if.
- + auto => /> &1 &2 Hrng ? Hh2 ???????????.
+ + auto => /> &2 Hrng ? Hh2 ?????????.
    have  /= Hrngp := decoded_unflattenE i{2} j{2} hint_0{2} (fun (ii : W32.t) => 0 <= to_uint ii < 2) _ _ _ _;1..4:smt().
    have  /= Hh2p := decoded_unflattenP i{2} j{2} hint_0{2} _hint (fun (ii : W32.t) => incoeff (to_uint ii)) _ _ _ _;1..4: smt(). 
    rewrite /(`<<`) /= /decoded_unflatten initiE 1:/# /=.
@@ -220,16 +341,18 @@ if.
    rewrite mulrC -Hh2p => H.
    by rewrite !to_uint_eq /=;smt( incoeffK).
 
- + auto => /> &1 &2 ???????????????Hone; do split; 1..2,5..6,9:smt(get_setE size_put). 
+ + auto => /> &1 &2 ????????????Hone; do split; 1..2,5..6,8:smt(Array3309.get_setE size_put). 
    + by smt(count_nonzero_prefix_one). 
    + move : Hone;rewrite /decoded_unflatten /count_nonzero_prefix ifT 1:/# ifT 1:/# /= (take_nth witness);1: by rewrite size_to_list /#.
      rewrite initiE 1:/# /= get_of_list 1:/# nth_sub 1:/# /= => -> /=.
      by rewrite -cats1 count_cat /= /#.
-   + smt(get_setE size_put nth_put). 
-   + move => k kbl kbh; rewrite nth_put; 1:by smt(count_nonzero_prefix_one).
-     case (count_nonzero_prefix (decoded_unflatten _hint) i{2} j{2} = w_hint + k);  smt(get_setE). 
-+ auto => /> &1 &2 ???????????????Hone; do split; 2..:smt().
+   + apply (eq_from_nth witness);1:smt(size_put size_mkseq).
+     move => k; rewrite size_put size_mkseq /max ifT 1:/# /= => kb.
+     by rewrite nth_put 1:/# /=; smt(nth_mkseq Array3309.get_setE).
++ auto => /> &1 &2 ????????????Hone; do split; 2..:smt().
    + move : Hone;rewrite /decoded_unflatten /count_nonzero_prefix ifT 1:/# ifT 1:/# /=  (take_nth witness);1: by rewrite size_to_list /#.
      rewrite initiE 1:/# /= get_of_list 1:/# nth_sub 1:/# /=.
      by rewrite -cats1 count_cat /= /#.
 qed.
+
+
